dafny/play.dfy
@@ -1,0 +1,4 @@
+   method Main() {
+       var l := [1,2,3];
+       print(l[..|l|]);
+    }
